functorized Comp

src/Framework/Comp.v
@@ -25,235 +25,254 @@ Module C1 := ReflComp.
 (* Behavioral Refinement *)
 (* Linking Preservation *)
 
-Section Comp.
+Module M (AM : Annotate).
 
-  Definition Top_n n m := Cross (Cross (C0.Top_n n) Annotate.trans_correct_top) (C1.Top_n m).
+  Section Comp_n.
 
-  Definition V_n n m := Cross (Cross (C0.V_n n) (fun v1 v2 => forall k, Annotate.V k v1 v2)) (C1.V_n m).
+    Definition Top_n n m := Cross (Cross (C0.Top_n n) AM.trans_correct_top) (C1.Top_n m).
 
-  Definition R_n n m := Cross (Cross (C0.R_n n) (fun v1 v2 => forall k, Annotate.R k v1 v2)) (C1.R_n m).
+    Definition V_n n m := Cross (Cross (C0.V_n n) (fun v1 v2 => forall k, AM.V k v1 v2)) (C1.V_n m).
 
-  Definition G_n n m Γ1 Γ2 := Cross (Cross (C0.G_n n Γ1 Γ2) (fun ρ1 ρ2 => forall k, Annotate.G_top k Γ1 ρ1 Γ2 ρ2)) (C1.G_n m Γ1 Γ2).
+    Definition R_n n m := Cross (Cross (C0.R_n n) (fun v1 v2 => forall k, AM.R k v1 v2)) (C1.R_n m).
 
-  Lemma V_n_wf_val_r n m v1 v2:
-    V_n n m v1 v2 ->
-    wf_val v2.
-  Proof.
-    unfold V_n, Cross.
-    intros H.
-    destruct H as [v2' [[v1' [HC0 HA]] HC1]].
-    specialize (HA 0).
-    eapply Annotate.V_wf_val_r in HA; eauto.
-    edestruct C1.V_n_wf_val; eauto.
-  Qed.
+    Definition G_n n m Γ1 Γ2 := Cross (Cross (C0.G_n n Γ1 Γ2) (fun ρ1 ρ2 => forall k, AM.G_top k Γ1 ρ1 Γ2 ρ2)) (C1.G_n m Γ1 Γ2).
 
-  Lemma R_n_V_n n m v1 v2:
-    R_n n m (A0.Res v1) (A1.Res v2) ->
-    V_n n m v1 v2.
-  Proof.
-    unfold R_n, V_n, Cross.
-    intros H.
-    destruct H as [r2' [[r1' [HC0 HA]] HC1]].
-    apply C0.R_n_Res_inv in HC0.
-    destruct HC0 as [v1' [Heqv1' HC0]]; subst.
-    edestruct Annotate.R_res_inv_l as [v2' [Heqv2' _]]; eauto; subst.
-    eexists; split; eauto.
-    eapply C1.R_n_V_n; eauto.
-  Qed.
+    Lemma V_n_wf_val_r n m v1 v2:
+      V_n n m v1 v2 ->
+      wf_val v2.
+    Proof.
+      unfold V_n, Cross.
+      intros H.
+      destruct H as [v2' [[v1' [HC0 HA]] HC1]].
+      specialize (HA 0).
+      eapply AM.V_wf_val_r in HA; eauto.
+      edestruct C1.V_n_wf_val; eauto.
+    Qed.
 
-  Lemma R_n_Res_inv n m v1 r2 :
-    R_n n m (A0.Res v1) r2 ->
-    exists v2, r2 = A1.Res v2 /\ V_n n m v1 v2.
-  Proof.
-    unfold R_n, V_n, Cross.
-    intros.
-    destruct H as [r2' [[r1' [HC0 HA]] HC1]].
-    apply C0.R_n_Res_inv in HC0.
-    destruct HC0 as [v1' [Heqv1' HC0]]; subst.
-    edestruct Annotate.R_res_inv_l as [v2' [Heqv2' HV]]; eauto; subst.
+    Lemma R_res_inv_l v1 r2 :
+      (forall i, AM.R i (A0.Res v1) r2) ->
+      exists v2, r2 = A1.Res v2 /\ (forall i, AM.V i v1 v2).
+    Proof.
+      intros.
+      pose proof (H 0) as H0.
+      eapply AM.R_res_inv_l in H0.
+      destruct H0 as [v2 [Heqv2 _]]; subst.
+      eexists; split; eauto.
+      intros.
+      specialize (H i).
+      apply AM.R_res_inv_l in H.
+      destruct H as [v2' [Heqv2' HV]]; inv Heqv2'; eauto.
+    Qed.
 
-    apply C1.R_n_Res_inv in HC1.
-    2 : { specialize (HV 0).
-          eapply Annotate.V_wf_val_r; eauto. }
-    destruct HC1 as [v2'' [Heqv2'' HC1]]; subst.
-    eexists; split; eauto.
-  Qed.
+    Lemma R_n_V_n n m v1 v2:
+      R_n n m (A0.Res v1) (A1.Res v2) ->
+      V_n n m v1 v2.
+    Proof.
+      unfold R_n, V_n, Cross.
+      intros H.
+      destruct H as [r2' [[r1' [HC0 HA]] HC1]].
+      apply C0.R_n_Res_inv in HC0.
+      destruct HC0 as [v1' [Heqv1' HC0]]; subst.
+      edestruct R_res_inv_l as [v2' [Heqv2' HV]]; eauto; subst.
+      eexists; split; eauto.
+      eapply C1.R_n_V_n; eauto.
+    Qed.
 
-  Lemma Top_n_subset n m e1 e2 :
-    Top_n n m e1 e2 ->
-    A1.occurs_free e2 \subset A0.occurs_free e1.
-  Proof.
-    unfold Top_n, Cross.
-    intros H.
-    destruct H as [e2' [[e1' [HC0 HA]] HC1]].
-    apply C0.Top_n_subset in HC0.
-    apply C1.Top_n_subset in HC1.
-    apply Annotate.trans_correct_top_subset in HA.
-    eapply Included_trans; eauto.
-    eapply Included_trans; eauto.
-  Qed.
+    Lemma R_n_Res_inv n m v1 r2 :
+      R_n n m (A0.Res v1) r2 ->
+      exists v2, r2 = A1.Res v2 /\ V_n n m v1 v2.
+    Proof.
+      unfold R_n, V_n, Cross.
+      intros.
+      destruct H as [r2' [[r1' [HC0 HA]] HC1]].
+      apply C0.R_n_Res_inv in HC0.
+      destruct HC0 as [v1' [Heqv1' HC0]]; subst.
+      edestruct R_res_inv_l as [v2' [Heqv2' HV]]; eauto; subst.
 
-  Lemma G_n_wf_env { n m Γ1 Γ2 ρ1 ρ2 } :
-    G_n n m Γ1 Γ2 ρ1 ρ2 ->
-    wf_env ρ2.
-  Proof.
-    unfold G_n, Cross.
-    intros H.
-    destruct H as [ρ2' [[ρ1' [HC0 HA]] HC1]].
-    specialize (HA 0).
-    apply Annotate.G_top_wf_env_r in HA.
-    eapply (C1.G_n_wf_env HC1); eauto.
-  Qed.
+      apply C1.R_n_Res_inv in HC1.
+      2 : { specialize (HV 0).
+            eapply AM.V_wf_val_r; eauto. }
+      destruct HC1 as [v2'' [Heqv2'' HC1]]; subst.
+      eexists; split; eauto.
+    Qed.
 
-  Lemma G_n_subset n m Γ1 Γ2 ρ1 Γ3 Γ4 ρ2 :
-    G_n n m Γ1 Γ2 ρ1 ρ2 ->
-    Γ3 \subset Γ1 ->
-    Γ4 \subset Γ3 ->
-    G_n n m Γ3 Γ4 ρ1 ρ2.
-  Proof.
-    unfold G_n, Cross.
-    intros H.
-    destruct H as [ρ2' [[ρ1' [HC0 HA]] HC1]].
+    Lemma Top_n_subset n m e1 e2 :
+      Top_n n m e1 e2 ->
+      A1.occurs_free e2 \subset A0.occurs_free e1.
+    Proof.
+      unfold Top_n, Cross.
+      intros H.
+      destruct H as [e2' [[e1' [HC0 HA]] HC1]].
+      apply C0.Top_n_subset in HC0.
+      apply C1.Top_n_subset in HC1.
+      apply AM.trans_correct_top_subset in HA.
+      eapply Included_trans; eauto.
+      eapply Included_trans; eauto.
+    Qed.
 
-    intros.
-    eapply C0.G_n_subset in HC0; eauto.
-    eapply C1.G_n_subset in HC1; eauto.
-    eexists; split; eauto.
-    eexists; split; eauto.
+    Lemma G_n_wf_env { n m Γ1 Γ2 ρ1 ρ2 } :
+      G_n n m Γ1 Γ2 ρ1 ρ2 ->
+      wf_env ρ2.
+    Proof.
+      unfold G_n, Cross.
+      intros H.
+      destruct H as [ρ2' [[ρ1' [HC0 HA]] HC1]].
+      specialize (HA 0).
+      apply AM.G_top_wf_env_r in HA.
+      eapply (C1.G_n_wf_env HC1); eauto.
+    Qed.
 
-    intros.
-    specialize (HA k).
-    eapply Annotate.G_top_subset; eauto.
-  Qed.
+    Lemma G_n_subset n m Γ1 Γ2 ρ1 Γ3 Γ4 ρ2 :
+      G_n n m Γ1 Γ2 ρ1 ρ2 ->
+      Γ3 \subset Γ1 ->
+      Γ4 \subset Γ3 ->
+      G_n n m Γ3 Γ4 ρ1 ρ2.
+    Proof.
+      unfold G_n, Cross.
+      intros H.
+      destruct H as [ρ2' [[ρ1' [HC0 HA]] HC1]].
 
-End Comp.
+      intros.
+      eapply C0.G_n_subset in HC0; eauto.
+      eapply C1.G_n_subset in HC1; eauto.
+      eexists; split; eauto.
+      eexists; split; eauto.
 
-Section Adequacy.
+      intros.
+      specialize (HA k).
+      eapply AM.G_top_subset; eauto.
+    Qed.
 
-  Lemma Top_n_R_n n m e1 e2:
-    Top_n n m e1 e2 ->
-    forall ρ1 ρ2,
-      wf_env ρ2 ->
-      G_n n m (A0.occurs_free e1) (A1.occurs_free e2) ρ1 ρ2 ->
-      forall j1 r1,
-        A0.bstep_fuel ρ1 e1 j1 r1 ->
-        exists j2 r2,
-          A1.bstep_fuel true ρ2 e2 j2 r2 /\
-          R_n n m r1 r2.
-  Proof.
-    intros Hrel.
-    unfold Top_n, G_n, R_n, Cross in *.
-    destruct Hrel as [e2' [[e1' [HC0 HA]] HC1]].
-    intros.
+  End Comp_n.
 
-    destruct H0 as [ρ2' [[ρ1' [HG0 HAG]] HG1]].
-    edestruct (C0.Top_n_R_n _ _ _ HC0) with (ρ2 := ρ1') as [j1' [r1' [Hstep1' HRn0]]]; eauto.
-    eapply C0.G_n_subset; eauto.
-    apply Included_refl.
-    eapply C0.Top_n_subset; eauto.
+  Section Adequacy.
 
-    assert (wf_env ρ2').
-    {
-      specialize (HAG 0).
-      eapply Annotate.G_top_wf_env_r; eauto.
-    }
+    Lemma Top_n_R_n n m e1 e2:
+      Top_n n m e1 e2 ->
+      forall ρ1 ρ2,
+        wf_env ρ2 ->
+        G_n n m (A0.occurs_free e1) (A1.occurs_free e2) ρ1 ρ2 ->
+        forall j1 r1,
+          A0.bstep_fuel ρ1 e1 j1 r1 ->
+          exists j2 r2,
+            A1.bstep_fuel true ρ2 e2 j2 r2 /\
+              R_n n m r1 r2.
+    Proof.
+      intros Hrel.
+      unfold Top_n, G_n, R_n, Cross in *.
+      destruct Hrel as [e2' [[e1' [HC0 HA]] HC1]].
+      intros.
 
-    edestruct (Annotate.adequacy _ _ HA) with (ρ2 := ρ2') as [j2' [r2' [Hstep2' HAR]]]; eauto.
-    - intros.
-      specialize (HAG k).
-      eapply Annotate.G_top_subset; eauto.
+      destruct H0 as [ρ2' [[ρ1' [HG0 HAG]] HG1]].
+      edestruct (C0.Top_n_R_n _ _ _ HC0) with (ρ2 := ρ1') as [j1' [r1' [Hstep1' HRn0]]]; eauto.
+      eapply C0.G_n_subset; eauto.
+      apply Included_refl.
       eapply C0.Top_n_subset; eauto.
-      eapply Annotate.trans_correct_top_subset; eauto.
-    - edestruct (C1.Top_n_R_n _ _ _ HC1) with (ρ2 := ρ2) as [j2 [r2 [Hstep2 HRn1]]]; eauto.
-      eapply C1.G_n_subset; eauto.
-      + eapply Annotate.trans_correct_top_subset in HA; eauto.
-        eapply Included_trans; eauto.
+
+      assert (wf_env ρ2').
+      {
+        specialize (HAG 0).
+        eapply AM.G_top_wf_env_r; eauto.
+      }
+
+      edestruct (AM.adequacy _ _ HA) with (ρ2 := ρ2') as [j2' [r2' [Hstep2' HAR]]]; eauto.
+      - intros.
+        specialize (HAG k).
+        eapply AM.G_top_subset; eauto.
         eapply C0.Top_n_subset; eauto.
-      + eapply C1.Top_n_subset; eauto.
-      + eexists; eexists; split; eauto.
-  Qed.
+        eapply AM.trans_correct_top_subset; eauto.
+      - edestruct (C1.Top_n_R_n _ _ _ HC1) with (ρ2 := ρ2) as [j2 [r2 [Hstep2 HRn1]]]; eauto.
+        eapply C1.G_n_subset; eauto.
+        + eapply AM.trans_correct_top_subset in HA; eauto.
+          eapply Included_trans; eauto.
+          eapply C0.Top_n_subset; eauto.
+        + eapply C1.Top_n_subset; eauto.
+        + eexists; eexists; split; eauto.
+    Qed.
 
-  (* Termination Perservation *)
-  Theorem Top_n_preserves_termination n m e1 e2 :
-    Top_n n m e1 e2 ->
-    forall ρ1 ρ2,
-      wf_env ρ2 ->
-      G_n n m (A0.occurs_free e1) (A1.occurs_free e2) ρ1 ρ2 ->
-      forall j1 v1,
-        A0.bstep_fuel ρ1 e1 j1 (A0.Res v1) ->
-        exists j2 v2,
-          A1.bstep_fuel true ρ2 e2 j2 (A1.Res v2) /\
-          V_n n m v1 v2.
-  Proof.
-    intros.
-    edestruct Top_n_R_n with (ρ1 := ρ1) as [j2 [r2 [Hr2 HR]]]; eauto.
-    edestruct R_n_Res_inv as [v2 [Heq HVn]]; eauto; subst.
-    eexists; eexists; split; eauto.
-  Qed.
+    (* Termination Perservation *)
+    Theorem Top_n_preserves_termination n m e1 e2 :
+      Top_n n m e1 e2 ->
+      forall ρ1 ρ2,
+        wf_env ρ2 ->
+        G_n n m (A0.occurs_free e1) (A1.occurs_free e2) ρ1 ρ2 ->
+        forall j1 v1,
+          A0.bstep_fuel ρ1 e1 j1 (A0.Res v1) ->
+          exists j2 v2,
+            A1.bstep_fuel true ρ2 e2 j2 (A1.Res v2) /\
+              V_n n m v1 v2.
+    Proof.
+      intros.
+      edestruct Top_n_R_n with (ρ1 := ρ1) as [j2 [r2 [Hr2 HR]]]; eauto.
+      edestruct R_n_Res_inv as [v2 [Heq HVn]]; eauto; subst.
+      eexists; eexists; split; eauto.
+    Qed.
 
-End Adequacy.
+  End Adequacy.
 
-Section Refinement.
+  Section Refinement.
 
-  Definition val_ref := Cross (Cross C0.val_ref Annotate.val_ref) C1.val_ref.
+    Definition val_ref := Cross (Cross C0.val_ref AM.val_ref) C1.val_ref.
 
-  Lemma R_n_res_val_ref {n m v1 v2} :
-    R_n n m (A0.Res v1) (A1.Res v2) ->
-    val_ref v1 v2.
-  Proof.
-    unfold R_n, val_ref, Cross.
-    intros.
-    destruct H as [r2' [[r1' [HC0 HR]] HC1]].
-    edestruct C0.R_n_Res_inv as [v1' [Heqv1' HV1]]; eauto; subst.
-    eapply C0.R_n_res_val_ref in HC0; eauto.
-    edestruct Annotate.R_res_inv_l as [v2' [Heqv2' HV2]]; eauto; subst.
-    eapply C1.R_n_res_val_ref in HC1; eauto.
-    eexists; split; eauto.
-    - eexists; split; eauto.
-      eapply Annotate.V_val_ref; eauto.
-    - specialize (HV2 0).
-      eapply Annotate.V_wf_val_r; eauto.
-  Qed.
+    Lemma R_n_res_val_ref {n m v1 v2} :
+      R_n n m (A0.Res v1) (A1.Res v2) ->
+      val_ref v1 v2.
+    Proof.
+      unfold R_n, val_ref, Cross.
+      intros.
+      destruct H as [r2' [[r1' [HC0 HR]] HC1]].
+      edestruct C0.R_n_Res_inv as [v1' [Heqv1' HV1]]; eauto; subst.
+      eapply C0.R_n_res_val_ref in HC0; eauto.
+      edestruct R_res_inv_l as [v2' [Heqv2' HV2]]; eauto; subst.
+      eapply C1.R_n_res_val_ref in HC1; eauto.
+      eexists; split; eauto.
+      - eexists; split; eauto.
+        eapply AM.V_val_ref; eauto.
+      - specialize (HV2 0).
+        eapply AM.V_wf_val_r; eauto.
+    Qed.
 
-  (* Behavioral Refinement *)
-  Theorem Top_n_val_ref n m e1 e2 :
-    Top_n n m e1 e2 ->
-    forall ρ1 ρ2,
-      wf_env ρ2 ->
-      G_n n m (A0.occurs_free e1) (A1.occurs_free e2) ρ1 ρ2 ->
-      forall j1 v1,
-        A0.bstep_fuel ρ1 e1 j1 (A0.Res v1) ->
-        exists j2 v2,
-          A1.bstep_fuel true ρ2 e2 j2 (A1.Res v2) /\
-          val_ref v1 v2.
-  Proof.
-    intros.
-    edestruct Top_n_R_n with (ρ1 := ρ1) as [j2 [r2 [Hr2 HR]]]; eauto.
-    edestruct R_n_Res_inv as [v2 [Heq HVn]]; eauto; subst.
-    eexists; eexists; split; eauto.
-    eapply R_n_res_val_ref; eauto.
-  Qed.
+    (* Behavioral Refinement *)
+    Theorem Top_n_val_ref n m e1 e2 :
+      Top_n n m e1 e2 ->
+      forall ρ1 ρ2,
+        wf_env ρ2 ->
+        G_n n m (A0.occurs_free e1) (A1.occurs_free e2) ρ1 ρ2 ->
+        forall j1 v1,
+          A0.bstep_fuel ρ1 e1 j1 (A0.Res v1) ->
+          exists j2 v2,
+            A1.bstep_fuel true ρ2 e2 j2 (A1.Res v2) /\
+              val_ref v1 v2.
+    Proof.
+      intros.
+      edestruct Top_n_R_n with (ρ1 := ρ1) as [j2 [r2 [Hr2 HR]]]; eauto.
+      edestruct R_n_Res_inv as [v2 [Heq HVn]]; eauto; subst.
+      eexists; eexists; split; eauto.
+      eapply R_n_res_val_ref; eauto.
+    Qed.
 
-End Refinement.
+  End Refinement.
 
-Section Linking.
+  Section Linking.
 
-  (* Linking Preservation *)
-  Lemma Top_n_preserves_linking f w x n n' m m' e1 e2 e1' e2' :
-    (w \in Exposed) ->
-    Top_n n m e1 e2 ->
-    Top_n n' m' e1' e2' ->
-    Top_n (n + n') (m + m') (A0.link f x e1 e1') (A1.link f w x e2 e2').
-  Proof.
-    unfold Top_n, Cross.
-    intro Hw.
-    intros.
-    destruct H as [e3 [[e4 [HC0 HA1]] HC1]].
-    destruct H0 as [e3' [[e4' [HC0' HA1']] HC1']].
+    (* Linking Preservation *)
+    Lemma Top_n_preserves_linking f w x n n' m m' e1 e2 e1' e2' :
+      (w \in Exposed) ->
+      Top_n n m e1 e2 ->
+      Top_n n' m' e1' e2' ->
+      Top_n (n + n') (m + m') (A0.link f x e1 e1') (A1.link f w x e2 e2').
+    Proof.
+      unfold Top_n, Cross.
+      intro Hw.
+      intros.
+      destruct H as [e3 [[e4 [HC0 HA1]] HC1]].
+      destruct H0 as [e3' [[e4' [HC0' HA1']] HC1']].
 
-    eapply (C0.Top_n_preserves_linking f x n n') in HC0; eauto.
-    eapply (Annotate.preserves_linking f w x e4 e3 e4' e3') in HA1; eauto.
-    eapply (C1.Top_n_preserves_linking f w x m m') in HC1; eauto.
-  Qed.
+      eapply (C0.Top_n_preserves_linking f x n n') in HC0; eauto.
+      eapply (AM.preserves_linking f w x e4 e3 e4' e3') in HA1; eauto.
+      eapply (C1.Top_n_preserves_linking f w x m m') in HC1; eauto.
+    Qed.
 
-End Linking.
+  End Linking.
+
+End M.
